% !TEX encoding = UTF-8 Unicode
%----------------------------------------
\documentclass[english,12pt,a4paper]{article}
%----------------------------------------
%
%----------------------------------------
\input{../packages}
\input{../macros.tex}
%====================================================

\title{Gradient methods}
\author{Roland Becker}
\date{\today}
\usepackage{environ}



%====================================================
\begin{document}
%====================================================
\maketitle
\setcounter{tocdepth}{2}
\tableofcontents
%
%
%==========================================
\section{Class of methods}\label{sec:}
%==========================================
%
%---------------------------------------
\begin{lemma}\label{lemma:}
Let $q_i(x) = q_i^* + \frac{\mu}{2}\norm{x- v_i}^2$. Then for $\lambda\in[0,1]$ we have for $q_{\lambda} := (1-\lambda)q_0+ \lambda q_1$ the expression
%
\begin{equation}\label{eq:toto1}
%
(1-\lambda)q_0(x) + \lambda q_1(x) = q_{\lambda}^* + \frac{\mu}{2}\norm{x- v_{\lambda}}^2
\end{equation}
%
with
%
\begin{equation}\label{eq:toto2}
v_{\lambda} = (1-\lambda)v_0 + \lambda v_1,\quad q_{\lambda}^* = (1-\lambda)q_0^* + \lambda q_1^* + \frac{\lambda(1-\lambda)\mu}{2}\norm{v_1-v_0}^2.
\end{equation}
%
Furthermore
%
\begin{equation}\label{eq:}
\argmin\SetDef{q^*_{\lambda}}{0\le \lambda\le1} = P_{[0,1]}\left(\frac12 + \frac{q_1^*-q_0^*}{\mu\norm{v_1-v_0}^2}\right).
\end{equation}
%
\end{lemma}
%
%---------------------------------------
\begin{proof}
The two functions in (\ref{eq:toto1}) are quadratic un $x$ and $\lambda$. Since they coincide for $\lambda=0$ and $\lambda=1$, it is sufficient to check that the second derivative with respect to $\lambda$ of the right-hand side vanishes:
%
\begin{align*}
\frac{\partial^2}{\partial \lambda^2}\norm{x-v_\lambda}^2 = 2\norm{v_1-v_0}^2 = -\frac{\partial^2\lambda(1-\lambda)}{\partial \lambda^2} \norm{v_1-v_0}^2
\end{align*}
%
\end{proof}
%

For $f\in\mathcal F_{\mu,L}(X)$ we  have
%
\begin{align*}
f(x) \ge f(y) + \scp{\nabla f(y)}{x-y} + \frac{\mu}{2}\norm{x-y}^2 = f(y) - \frac{1}{2\mu}\norm{\nabla f(y)}^2 + \frac{\mu}{2}\norm{x-y+\frac{1}{\mu}\nabla f(y)}^2
\end{align*}
%

%
\begin{yellow}
\begin{algorithm}[H]
\caption{GM fixed step size} 
\label{algorithm:AGMfixed} 
%
Input: $x_0\in X$, $\eps>0$.\\ Set $v_{0}=x_0$, $q_0=-\infty$ and $k=0$.
%
\begin{itemize}
\item[(1)] If $f(x_k)-q_k \le \eps$: STOP
\item[(5)] $x_{k+1} = x_k  - \frac{1}{L}\nabla f(x_k)$
\item[(3)] $w_k=x_k - \frac{1}{\mu}\nabla f(x_k)$,  $p_k=f(x_k) - \frac{\norm{\nabla f(x_k)}^2}{2\mu}$
\item[] $Q_{k} = \frac{\mu}{2}\norm{v_k -w_k}^2$, $\lambda_{k} = P_{[0,1]}\left(\frac12 + \frac{p_k-q_k}{2Q_k}\right)$
\item[] $q_{k+1} = (1-\lambda_k) q_k + \lambda_k p_k + \lambda_k(1-\lambda_k)Q_{k}$
\item[(4)] $v_{k+1} = (1-\lambda_k) v_{k} + \lambda_k w_k$
\item[(6)] Increment $k$ and go to (1)
\end{itemize}
%
\end{algorithm}
\end{yellow}
%

%
\begin{yellow}
\begin{algorithm}[H]
\caption{AGM fixed step size} 
\label{algorithm:AGMfixed} 
%
Input: $x_0\in X$, $\eps>0$.\\ Set $v_{0}=x_0- \frac{1}{\mu}\nabla f(x_0)$, $q_0=f(x_0) - \frac{\norm{\nabla f(x_0)}^2}{2\mu}$ and $k=0$.
%
\begin{itemize}
\item[(1)] If $f(x_k)-q_k \le \eps$: STOP
\item[(2)] $y_{k} = (1-\theta_k)v_k + \theta_k x_{k}$
\item[(3)] $Q_{k} = \frac{\mu}{2}\norm{v_k -y_k + \frac{1}{\mu}\nabla f(y_k)}^2$
\item[] $q_{k+1} = (1-\lambda_k) q_k + \lambda_k\left(  f(y_k) - \frac{\norm{\nabla f(y_k)}^2}{2\mu}\right) + \lambda_k(1-\lambda_k)Q_{k}$
\item[(4)] $v_{k+1} = (1-\lambda_k) v_{k} + \lambda_k \left( y_k - \frac{1}{\mu}\nabla f(y_k)\right)$
\item[(5)] $x_{k+1} = y_{k}  - \frac{1}{L}\nabla f(y_k)$
\item[(6)] Increment $k$ and go to (1)
\end{itemize}
%
\end{algorithm}
\end{yellow}
%

For $\theta_k<1$ we have 
%
\begin{align*}
v_k -y_k = \frac{\theta_k}{1-\theta_k}(y_k-x_k)
\end{align*}
%
such that
%
\begin{align*}
Q_{k} = \frac{\theta_k^2\mu}{2(1-\theta_k)^2}\norm{x_k -y_k}^2 + \frac{1}{2\mu}\norm{\nabla f(y_k)}^2+ \frac{\theta_k}{1-\theta_k}\scp{\nabla f(y_k)}{y_k -x_k}.
\end{align*}

Let $e_k:=f(x_k) -q_k$ Then we have

\begin{align*}
e_{k+1}\le& f(y_k) - \frac{1}{2L} \norm{\nabla f(y_k)}^2 - q_{k+1} & (5)\\
=&  (1-\lambda_k)(f(y_k) -q_k)  - \frac{1}{2L} \norm{\nabla f(y_k)}^2 + \lambda_k\frac{\norm{\nabla f(y_k)}^2}{2\mu} - \lambda_k(1-\lambda_k)Q_{k}\\
=&  (1-\lambda_k)e_k + \underbrace{(1-\lambda_k)\scp{\nabla f(y_k)}{y_k-x_k}  +\left(\frac{\lambda_k}{2\mu}- \frac{1}{2L}\right) \norm{\nabla f(y_k)}^2 - \lambda_k(1-\lambda_k)Q_{k}}_{=:X}
\end{align*}

%
\begin{align*}
X =& (1-\lambda_k)\left(1-\frac{\lambda_k\theta_k}{1-\theta_k}\right)\scp{\nabla f(y_k)}{y_k-x_k} + \left(\frac{\lambda_k}{2\mu}- \frac{1}{2L} - \frac{\lambda_k(1-\lambda_k)}{2\mu}\right) \norm{\nabla f(y_k)}^2 \\&- \frac{\lambda_k(1-\lambda_k)\theta_k^2\mu}{2(1-\theta_k)^2}\norm{x_k -y_k}^2\\
=& \frac{(1-\lambda_k)(1-(1+\lambda_k)\theta_k)}{1-\theta_k}\scp{\nabla f(y_k)}{y_k-x_k} + \left(\frac{\lambda_k^2}{2\mu}- \frac{1}{2L}\right) \norm{\nabla f(y_k)}^2 \\&- \frac{\lambda_k(1-\lambda_k)\theta_k^2\mu}{2(1-\theta_k)^2}\norm{x_k -y_k}^2
\end{align*}
%
Under the condition $(1+\lambda_k)\theta_k<1$ we get
%
\begin{align*}
X \le \left(\frac{2(1-\theta_k)^2}{4\lambda_k(1-\lambda_k)\theta_k^2\mu}\frac{(1-\theta_k)^2}{(1-\lambda_k)^2(1-(1+\lambda_k)\theta_k)^2} + \frac{\lambda_k^2}{2\mu}- \frac{1}{2L}\right) \norm{\nabla f(y_k)}^2
\end{align*}
%









%====================================================
%====================================================
\end{document}
%===================================================w